messageInvariantPrototypes/paxos/centralizedMonotonic_globalHistory/readme.md
@@ -1,7 +1,0 @@
-# Readme
-
-Monotonic version of Centralized Paxos.
-
-This is done by making the group of host a history in System.
-
-Note that the System.dfy spec is unchanged.
